src/tactic/vampire/compile.lean
@@ -16,34 +16,60 @@ namespace vampire
 
 open tactic
 
-def disjoiner (c d : cla) : smaps :=
+
+@[derive decidable_eq]
+inductive inf : Type
+| hyp (k : nat) : inf
+| res : inf
+| rot (k : nat) : inf
+| sub (μ : mappings) : inf
+| con : inf
+
+namespace inf
+
+def repr : inf → string
+| (hyp k) := k.repr ++ " h"
+| res     := "r"
+| (rot k) := k.repr ++ " t"
+| (sub μ) := μ.repr ++ " s"
+| con     := "c"
+
+instance has_repr : has_repr inf := ⟨repr⟩
+
+meta instance has_to_format : has_to_format inf := ⟨λ x, repr x⟩
+
+end inf
+
+@[reducible] def infs : Type := list inf
+
+def disjoiner (c d : cla) : mappings :=
 d.vars.map (λ k, (k, sum.inl $ k + c.fresh_var))
 
-meta def unifier : term → term → tactic smaps
+meta def unifier : term → term → tactic mappings
 | (term.sym k) (term.sym m) :=
   guard (k = m) >> return []
 | (term.app t1 t2) (term.app s1 s2) :=
   do μ ← unifier t2 s2,
      ν ← unifier (t1.subst μ) (s1.subst μ),
-     return (smaps.compose ν μ)
+     return (mappings.compose ν μ)
 | (term.app t1 t2) (term.vpp s k) :=
   do guard (¬ k ∈ t2.vars),
      μ ← unifier (t1.subst [(k, sum.inr t2)]) (s.subst [(k, sum.inr t2)]),
-     return (smaps.compose μ [(k, sum.inr t2)])
+     return (mappings.compose μ [(k, sum.inr t2)])
 | (term.vpp t k) (term.app s1 s2) :=
   do guard (¬ k ∈ s2.vars),
      μ ← unifier (t.subst [(k, sum.inr s2)]) (s1.subst [(k, sum.inr s2)]),
-     return (smaps.compose μ [(k, sum.inr s2)])
+     return (mappings.compose μ [(k, sum.inr s2)])
 | (term.vpp t k) (term.vpp s m) :=
   do μ ← unifier (t.subst [(m, sum.inl k)]) (s.subst [(m, sum.inl k)]),
-     return (smaps.compose μ [(m, sum.inl k)])
+     return (mappings.compose μ [(m, sum.inl k)])
 | t s := fail ("Nonunifiable terms : " ++ t.repr ++ " " ++ s.repr)
 
-meta def unifiers (δ : smaps) (t s : term) : tactic (smaps × smaps) :=
+meta def unifiers (δ : mappings) (t s : term) : tactic (mappings × mappings) :=
 do μ ← unifier t (s.subst δ),
-   return (μ, smaps.compose μ δ)
+   return (μ, mappings.compose μ δ)
 
-meta def instantiator.merge_core : smaps → smaps → smaps → tactic smaps
+meta def instantiator.merge_core : mappings → mappings → mappings → tactic mappings
 | [] μ ν             := return (μ ++ ν)
 | ((m, t) :: ξ) μ ν  :=
   match ν.find (λ x, prod.fst x = m) with
@@ -54,10 +80,10 @@ meta def instantiator.merge_core : smaps → smaps → smaps → tactic smaps
     else failed
   end
 
-meta def instantiator.merge : smaps → smaps → tactic smaps
+meta def instantiator.merge : mappings → mappings → tactic mappings
 | μ ν := instantiator.merge_core μ [] ν
 
-meta def term.instantiator : term → term → tactic smaps
+meta def term.instantiator : term → term → tactic mappings
 | (term.sym k) (term.sym m) :=
   guard (k = m) >> return []
 | (term.app t1 t2) (term.app s1 s2) :=
@@ -72,7 +98,7 @@ meta def term.instantiator : term → term → tactic smaps
      instantiator.merge μ [(k, sum.inl m)]
 | _ _ := fail "RHS is not an instance of LHS"
 
-meta def cla.instantiator : cla → cla → tactic smaps
+meta def cla.instantiator : cla → cla → tactic mappings
 | [] [] := return []
 | ((a, t) :: c) ((b, s) :: d) :=
   if a = b
@@ -101,30 +127,30 @@ instance is_dup.decidable : decidable_pred is_dup
 meta def tactic.guard (p : Prop) [decidable p] (s : string) : tactic unit :=
 if p then skip else trace s >> failed
 
-meta def allign_premises (π1 π2 : expr) :
-  cla → cla → tactic (expr × expr × term × term × cla × cla)
-| ((ff, t1) :: c1) ((tt, t2) :: c2) := return (π1, π2, t1, t2, c1, c2)
-| ((tt, t1) :: c1) ((ff, t2) :: c2) := return (π2, π1, t2, t1, c2, c1)
+meta def allign_premises (ifs1 ifs2 : infs) :
+  cla → cla → tactic (infs × infs × term × term × cla × cla)
+| ((ff, t1) :: c1) ((tt, t2) :: c2) := return (ifs1, ifs2, t1, t2, c1, c2)
+| ((tt, t1) :: c1) ((ff, t2) :: c2) := return (ifs2, ifs1, t2, t1, c2, c1)
 | _ _ := failed
 
-meta def rots (mx πx : expr) (c : cla) : list (expr × cla) :=
+meta def rots (ifs : infs) (c : cla) : list (infs × cla) :=
 (list.range c.length).map
-  (λ x, (expr.mk_app `(@proof.rot) [mx, x.to_expr, c.to_expr, πx], c.rot x))
+  (λ x, (ifs ++ [inf.rot x], c.rot x))
 
-meta def lit.unifier : lit → lit → tactic smaps
+meta def lit.unifier : lit → lit → tactic mappings
 | (a, t) (b, s) :=
   if a = b
   then unifier t s
   else failed
 
-meta def lit.instantiator : lit → lit → tactic smaps
+meta def lit.instantiator : lit → lit → tactic mappings
 | (a, t) (b, s) :=
   if a = b
   then term.instantiator t s
   else failed
 
 meta def compute_map (d : cla) :
-  cla → smaps → list nat → nat → tactic (smaps × list nat)
+  cla → mappings → list nat → nat → tactic (mappings × list nat)
 | [] μ ns _ :=
   if ∀ x < d.length, x ∈ ns
   then return (μ, ns.reverse)
@@ -152,78 +178,84 @@ def remove_nth' {α : Type} : list α → ℕ → option (list α)
   do xs' ← remove_nth' xs k,
      some (x :: xs')
 
-meta def compile_cnts_aux (mx : expr) :
-  expr → list nat → cla → tactic (expr × list nat × cla)
-| πx (k :: ks) (l :: c) :=
+meta def compile_cnts_aux :
+  list nat → cla → tactic (infs × list nat × cla)
+| (k :: ks) (l :: c) :=
   ( do n ← index_of' k ks,
        ks' ← remove_nth' ks n,
        c'  ← remove_nth' c n,
-       let πx'  : expr := expr.mk_app `(@proof.rot) [mx, (n + 1).to_expr, cla.to_expr (l :: c), πx],
-       let πx'' : expr := expr.mk_app `(@proof.con) [mx, l.to_expr, cla.to_expr c', πx'],
-       compile_cnts_aux πx'' (k :: ks') (l :: c') ) <|>
-  ( return (πx, k :: ks, l :: c))
-| _ _ _ := failed
+       (ifs, ks'', c'') ← compile_cnts_aux (k :: ks') (l :: c'),
+       return ((inf.rot (n + 1) :: inf.con :: ifs), ks'', c'') ) <|>
+  ( return ([], k :: ks, l :: c) )
+| _ _ := failed
 
-meta def compile_cnts (mx : expr) (d : cla)  :
-  nat → expr → (list nat) → cla → tactic (expr × cla)
-| 0 πx _ c :=
+meta def compile_cnts (d : cla) :
+  nat → list nat → cla → tactic (infs × cla)
+| 0 _ c :=
   do tactic.guard (list.exteq c d)
      "Contraction result not equivalent to target", -- To do : remove when compiler is reliable
-     return (πx, c)
-| (k + 1) πx ns c :=
-  do i ← index_of' k ns,
-     let πx' : expr := expr.mk_app `(@proof.rot) [mx, i.to_expr, c.to_expr, πx],
-     (πx'', ns', c') ← compile_cnts_aux mx πx' (ns.rot i) (c.rot i),
-     compile_cnts k πx'' ns' c'
+     return ([], c)
+| (k + 1) ks c :=
+  do i ← index_of' k ks,
+     (ifs1, ks', c') ← compile_cnts_aux (ks.rot i) (c.rot i),
+     (ifs2, c'') ← compile_cnts k ks' c',
+     return ((inf.rot i :: (ifs1 ++ ifs2)), c'')
 
-meta def compile_map (mx πx : expr) (c d : cla) : tactic (expr × cla) :=
+
+def cons_sub : mappings → infs → infs
+| [] is := is
+| μ  is := inf.sub μ :: is
+
+meta def compile_map (c d : cla) : tactic (infs × cla) :=
 do let δ  := disjoiner d c,
    let cδ := c.subst δ,
-   let σx := expr.mk_app `(@proof.sub) [mx, δ.to_expr, c.to_expr, πx],
-   (μ, ns) ← compute_map d cδ [] [] d.length,
+   (μ, ks) ← compute_map d cδ [] [] d.length,
    let cδμ := cδ.subst μ,
-   let τx : expr := expr.mk_app `(@proof.sub) [mx, μ.to_expr, cδ.to_expr, σx],
-   compile_cnts mx d d.length τx ns cδμ
+   (ifs, c') ← compile_cnts d d.length ks cδμ,
+   return (cons_sub δ (cons_sub μ ifs), c')
 
-meta def compile_res (mx : expr) (c : cla) :
-  list ((expr × cla) × (expr × cla)) → tactic (expr × cla)
+meta def compile_res (d : cla) :
+  list ((infs × cla) × (infs × cla)) → tactic (infs × cla)
 | [] := failed
-| (((π1, c1), (π2, c2)) :: l) :=
-  ( do (σ1, σ2, t1, t2, d1, d2) ← allign_premises π1 π2 c1 c2,
-       let e1 := ((ff, t1) :: d1),
-       let e2 := ((tt, t2) :: d2),
-       (μ, ν) ← unifiers (disjoiner e1 e2) t1 t2,
-       let σ1' : expr := expr.mk_app `(@proof.sub) [mx, μ.to_expr, cla.to_expr e1, σ1],
-       let σ2' : expr := expr.mk_app `(@proof.sub) [mx, ν.to_expr, cla.to_expr e2, σ2],
-       let t   : term := t1.subst μ,
-       let d1' : cla  := d1.subst μ,
-       let d2' : cla  := d2.subst ν,
-       let d   : cla  := d1' ++ d2',
-       let σ   : expr := expr.mk_app `(@proof.res)
-                         [mx, t.to_expr, d1'.to_expr, d2'.to_expr, σ1', σ2'],
-       compile_map mx σ d c ) <|>
+| (((is1, c1), (is2, c2)) :: l) :=
+  ( do (isl, isr, tl, tr, cl, cr) ← allign_premises is1 is2 c1 c2,
+       let tcl := ((ff, tl) :: cl),
+       let tcr := ((tt, tr) :: cr),
+       (μ, ν) ← unifiers (disjoiner tcl tcr) tl tr,
+       let isl' : infs := isl ++ [inf.sub μ],
+       let isr' : infs := isr ++ [inf.sub ν],
+       let t    : term := tl.subst μ,
+       let clμ  : cla  := cl.subst μ,
+       let crν  : cla  := cr.subst ν,
+       let c    : cla  := clμ ++ crν,
+       (is, c') ← compile_map c d,
+       return (isl' ++ isr' ++ (inf.res :: is), c') ) <|>
   ( compile_res l )
 
 meta def compile_core : list line →
-  mat → expr → nat → cla → rule → tactic (expr × cla)
-| ls m mx k c rule.inp :=
-  let d := m.nth (k - 1) in
-  compile_map mx (expr.mk_app `(@proof.hyp) [mx, (k - 1).to_expr]) d c
-| ls m mx k c (rule.map n) :=
-  do ⟨k', c', r⟩ ← find_line n ls,
-     (πx, d) ← compile_core ls m mx k' c' r,
-     compile_map mx πx d c
-| ls m mx k c (rule.res n1 n2) :=
-  do ⟨k1, c1, r1⟩ ← find_line n1 ls,
-     ⟨k2, c2, r2⟩ ← find_line n2 ls,
-     (π1, d1) ← compile_core ls m mx k1 c1 r1,
-     (π2, d2) ← compile_core ls m mx k2 c2 r2,
-     let ccs := list.product (rots mx π1 d1) (rots mx π2 d2),
-     compile_res mx c ccs
+  mat → nat → cla → rule → tactic (infs × cla)
+| ls m k d rule.inp :=
+  let c := m.nth (k - 1) in
+  do (is, c') ← compile_map c d,
+     trace (inf.hyp (k - 1) :: is),
+     return (inf.hyp (k - 1) :: is, c')
+| ls m k d (rule.map n) :=
+  do ⟨k', d', r⟩ ← find_line n ls,
+     (is1, c) ← compile_core ls m k' d' r,
+     (is2, c') ← compile_map c d,
+     return (is1 ++ is2, c')
+| ls m k d (rule.res n1 n2) :=
+  do ⟨k1, d1, r1⟩ ← find_line n1 ls,
+     ⟨k2, d2, r2⟩ ← find_line n2 ls,
+     (is1, c1) ← compile_core ls m k1 d1 r1,
+     (is2, c2) ← compile_core ls m k2 d2 r2,
+     let ccs := list.product (rots is1 d1) (rots is2 d2),
+     compile_res d ccs
 
-meta def compile (m : mat) (ls : list line) : tactic expr :=
+meta def compile (m : mat) (ls : list line) : tactic infs :=
 do ⟨k, [], r⟩ ← list.find (λ l, line.c l = []) ls,
-   (πx, _) ← compile_core ls m m.to_expr k [] r,
-   return πx
+   (is, _) ← compile_core ls m k [] r,
+   trace "Before filter : ", trace is,
+   return (is.filter (λ x, x ≠ inf.rot 0 ∧ x ≠ inf.sub []))
 
 end vampire
